src/lowparse/LowParse.SLow.Bytes.fst
@@ -83,3 +83,30 @@ let serialize32_bounded_vlbytes
     #serialize_all_bytes
     serialize32_all_bytes
     input
+
+#reset-options "--z3rlimit 32 --z3cliopt smt.arith.nl=false"
+
+inline_for_extraction
+let size32_all_bytes
+: size32 serialize_all_bytes
+= fun (input: B32.bytes) ->
+  let res = B32.len input in
+  (res <: (res: U32.t { size32_postcond serialize_all_bytes input res } ))
+
+inline_for_extraction
+let size32_bounded_vlbytes
+  (min: nat)
+  (max: nat { min <= max /\ max > 0 /\ max < 4294967292 } ) // max MUST BE less than 2^32 - 4
+  (size_header_byte_size32: U32.t { U32.v size_header_byte_size32 == log256' max } )
+: Tot (size32 (serialize_bounded_vlbytes min max))
+= fun (input: parse_bounded_vlbytes_t min max) ->
+  size32_bounded_vldata_strong
+    min
+    max
+    #_
+    #_
+    #parse_all_bytes
+    #serialize_all_bytes
+    size32_all_bytes
+    size_header_byte_size32
+    input
